examples/new_stack/NewStack23Aproof.v
@@ -1,4 +1,4 @@
-Require Import NewStack2 NewStack3A HoareDef SimModSem.
+Require Import NewStackHeader NewStack2 NewStack3A HoareDef SimModSem.
 Require Import Coqlib.
 Require Import Universe.
 Require Import Skeleton.
@@ -17,7 +17,7 @@ From ExtLib Require Import
      Data.Map.FMapAList.
 Require Import TODOYJ.
 Require Import HTactics Logic IPM.
-Require Import OpenDef.
+Require Import OpenDef STB.
 Require Import TODO.
 
 Set Implicit Arguments.
@@ -82,12 +82,21 @@ Section SIMMODSEM.
     (* Lemma update_wf: forall `{Dec K} (f: @URA.car RA) k v (WF: URA.wf f) (WF: URA.wf v), URA.wf (update f k v: (@URA.car RA)). *)
     (* Proof. ii. unfold update. des_ifs; ss. Qed. *)
 
-    Lemma pw_wf: forall (f: @URA.car RA) (WF: URA.wf f), <<WF: forall k, URA.wf (f k)>>.
+    Lemma pw_wf: forall (f: K -> M) (WF: URA.wf (f: @URA.car RA)), <<WF: forall k, URA.wf (f k)>>.
     Proof. ii; ss. rewrite URA.unfold_wf in WF. ss. Qed.
+
+    Lemma pw_insert_wf: forall `{EqDecision K} (f: K -> M) k v (WF: URA.wf (f: @URA.car RA)) (WFV: URA.wf v),
+        <<WF: URA.wf (<[k:=v]> f: @URA.car RA)>>.
+    Proof.
+      i. unfold insert, fn_insert. ur. ii. des_ifs. ur in WF. eapply WF.
+    Qed.
 
   End AUX.
 
-  Theorem sim_modsem: ModSemPair.sim (NewStack3A.StackSem) (NewStack2.StackSem).
+  Variable global_stb: list (string * fspec).
+  Hypothesis STBINCL: stb_incl (DebugStb ++ StackStb) global_stb.
+
+  Theorem sim_modsem: ModSemPair.sim (NewStack3A.StackSem global_stb) (NewStack2.StackSem).
   Proof.
     econstructor 1 with (wf:=wf); ss; et; swap 2 3.
     { econs; ss.
@@ -135,69 +144,60 @@ Section SIMMODSEM.
     }
     econs; ss.
     { unfold NewStack2.pop_body, cfun. init. harg. fold wf. des_ifs_safe. mDesAll. des; clarify.
-      apply Any.upcast_inj in PURE0. des; clarify. steps. rewrite Any.upcast_downcast in *. clarify. steps.
+      steps. rewrite Any.upcast_downcast in *. clarify. steps.
       astart 0. astop. steps. rewrite Any.upcast_downcast in *. clarify.
-      rename g into stk_mgr0. rename n into h. rename a1 into stk_res0.
+      rename g into stk_mgr0. rename n into h. rename a1 into stk_res0. rename varg_src into stk0.
       mCombine "A1" "A".
       mOwnWf "A1".
       assert(A: forall k, URA.wf ((stk_res0 k): URA.car (t:=Excl.t _))).
       { eapply URA.wf_mon in WF0.
         eapply Auth.black_wf in WF0. eapply pw_wf in WF0. des. ii. specialize (WF0 k). ss. }
-      assert(B: stk_res0 h = Some l).
+      assert(B: stk_res0 h = Some stk0).
       { dup WF0.
         eapply Auth.auth_included in WF0. des. unfold _is_stack in WF0. eapply pw_extends in WF0. des.
         spc WF0. des_ifs. ss. eapply Excl.extends in WF0; ss. }
       assert(C:=B). eapply SIM in C. rewrite C. steps.
-      destruct l as [|x stk].
-      - steps. force_l. esplits. steps. hret _; ss.
-        iDestruct "A1" as "[A B]".
-        iModIntro. iFrame. iSplit; ss; et.
-      - steps. Auth.auth_update
-      force_l. exists (Vptr h 0). steps.
-      mOwnWf "A".
-      assert(WF1: forall k, stk_res0 k <> Excl.boom).
-      { ur in WF0. des. r in WF1. repeat ur in WF1. rewrite Seal.sealing_eq in WF1. hexploit (WF1); et. }
+      destruct stk0 as [|x stk1].
+      - steps. hret _; ss. iDestruct "A1" as "[A B]". iModIntro. iFrame. iSplit; ss; et.
+      - steps.
+        destruct (alist_find "debug" (DebugStb ++ StackStb)) eqn:U; cycle 1.
+        { exfalso. stb_tac. ss. }
+        dup U. revert U. stb_tac. clarify. i.
+        apply STBINCL in U. rewrite U. steps. rewrite Any.upcast_downcast. steps.
 
-      hret _; ss.
-      { iPoseProof (OwnM_Upd with "A") as "A".
-        { eapply Auth.auth_alloc2. instantiate (1:=(_is_stack h [])).
-          ur. i. specialize (WF1 k).
-          destruct (dec k h).
-          - subst. ur.
-            destruct (stk_res0 h) eqn:T; ss.
-            + erewrite SIM in T. clarify.
-            + unfold _is_stack. des_ifs.
-          - ur.
-            destruct (stk_res0 k) eqn:T; ss.
-            + unfold _is_stack. des_ifs.
-            + unfold _is_stack. des_ifs.
+        set (stk_res1:=<[h:=Excl.just stk1]>stk_res0).
+        assert(WF1: URA.wf (stk_res1: URA.car (t:=_stkRA))).
+        { subst stk_res1. eapply (@pw_insert_wf _ (Excl.t (list Z))); et.
+          { eapply URA.wf_mon in WF0. eapply Auth.black_wf in WF0. ss. }
+          ur; ss.
         }
-        iMod "A". iDestruct "A" as "[A B]". iModIntro. iSplitL "A"; et.
-        iExists _, _. iSplit; ss; et. iSplit; ss; et. iPureIntro. ii.
-        assert(B: stk_res0 h = Excl.unit).
-        { destruct (stk_res0 h) eqn:T; ss.
-          - rewrite SIM in T. rewrite T in *. ss.
-          - exploit WF1; et; ss.
+
+        mAssert _ with "A1".
+        { iApply (OwnM_Upd with "A1").
+          eapply Auth.auth_update with (a':=stk_res1) (b':=_is_stack h (stk1)).
+          bar. ii. ss. des. clarify. esplits; et.
+          assert(D: ctx0 h = Excl.unit).
+          { clear - B. repeat ur in B. unfold _is_stack in *. des_ifs. }
+          extensionality h0. subst stk_res1. unfold insert, fn_insert. des_ifs. 
+          - ur. rewrite D. unfold _is_stack. ur. des_ifs.
+          - unfold _is_stack. ur. des_ifs.
         }
-        clear - SIM WF1 B.
-        destruct (dec h h0).
-        - subst. rewrite lookup_insert.
-          ur. ur. unfold _is_stack. des_ifs_safe. ss. clarify. split; i; clarify.
-        - rewrite lookup_insert_ne; ss.
-          ur. ur. unfold _is_stack. des_ifs_safe. ss. erewrite <- SIM. split; i; des_ifs.
-      }
-    }
+        mUpd "A". mDesOwn "A".
 
-    split; i.
+        assert(SIM0: ∀ h0 stk,
+                  <[h:=Excl.just stk1]> stk_res0 h0 = Excl.just stk ↔ <[h:=stk1]> stk_mgr0 !! h0 = Some stk).
+        { ii. destruct (dec h h0).
+          - subst. erewrite ! lookup_insert. unfold insert, fn_insert. des_ifs. split; i; clarify.
+          - erewrite ! lookup_insert_ne; ss. unfold insert, fn_insert. des_ifs. }
 
-          spc SIM. specialize (SIM []).
-          rewrite <- SIM. lookup rewrite fn_lookup_insert. ss.
-          ur.
-          { iPureIntro.
-      }
-      admit "mid - somehow".
+        hcall _ _ _ with "A"; ss; et.
+        { iModIntro. iSplit; ss. iExists _, stk_res1. iSplit; ss; et. }
+        { ss. }
+        steps. mDesAll. subst. des; clarify.
+
+        hret _; ss.
+        iModIntro. iFrame. iSplit; ss. iExists _, _; ss; et.
     }
-    admit "mid - somehow".
   Unshelve.
     all: ss.
   Qed.
