examples/new_stack/NewStackHeader.v
@@ -1,0 +1,31 @@
+Require Import Coqlib.
+Require Import ITreelib.
+Require Import Universe.
+Require Import STS.
+Require Import Behavior.
+Require Import ModSem.
+Require Import Skeleton.
+Require Import PCM.
+Require Import HoareDef.
+Require Import SimModSem.
+From ExtLib Require Import
+     Core.RelDec
+     Structures.Maps
+     Data.Map.FMapAList.
+Require Import Logic OpenDef.
+
+Set Implicit Arguments.
+
+Section PROOF.
+
+  Context `{Σ: GRA.t}.
+
+  Definition DebugStb: list (gname * fspec).
+   eapply (Seal.sealing "stb").
+   eapply [("debug", (mk_simple (X:=unit) (fun _ => ((fun _ o => (⌜o = ord_top⌝: iProp)%I),
+                                                     (fun _ => (⌜True⌝: iProp)%I)))))].
+  Defined.
+
+End PROOF.
+
+Global Hint Unfold DebugStb: stb.
